removed sorted

MQUM.v
@@ -45,9 +45,35 @@ Now we state our main theorems.
 
 Definition UM B A:=  
 replace_column 
-(UM_aux (sort by_dbp B) (sort by_sp A) 0 0) (uniform_price B A).
+(UM_aux (sort by_dbp B) (sort by_sp A) 0 0) (uniform_price (sort by_dbp B) (sort by_sp A)).
 
 
+
+
+          
+(*Bellow three lemmas can be moved to lower level*)
+Lemma idb_sort (B:list Bid): 
+NoDup (idbs_of B) -> NoDup (idbs_of (sort by_dbp B)).
+Proof. assert(perm (idbs_of B) (idbs_of (sort by_dbp B))). apply idb_perm.
+eauto. intros. eapply perm_nodup. eauto. eauto. Qed.
+
+
+Lemma ida_sort (A:list Ask): 
+NoDup (idas_of A) -> NoDup (idas_of (sort by_sp A)).
+Proof. assert(perm (idas_of A) (idas_of (sort by_sp A))). apply ida_perm.
+eauto. intros. eapply perm_nodup. eauto. eauto. Qed.
+
+Lemma fair_sort (M:list fill_type)(B:list Bid)(A:list Ask):
+Is_fair M (sort by_dbp B) (sort by_sp A) -> Is_fair M B A.
+Proof. unfold Is_fair. unfold fair_on_asks. unfold fair_on_bids.
+intros. destruct H. split. intros. split. apply H in H2.
+apply H2. destruct H1. split. eauto. eauto. auto. auto.
+apply H in H2.
+apply H2. destruct H1. split. eauto. eauto. auto. auto.
+intros. split. apply H0 in H2.
+apply H2. destruct H1. split. eauto. eauto. auto. auto.
+apply H0 in H2.
+apply H2. destruct H1. split. eauto. eauto. auto. auto. Qed.
 
 (*Following Theorem says the The processs UM is Individual Rational 
 and Uniform matching. Note that Is_uniform is defined as IR 
@@ -58,57 +84,89 @@ Theorem UM_Is_Uniform (B:list Bid)(A:list Ask)
 (NDA:NoDup (idas_of A))
 (NDB:NoDup (idbs_of B))
 (Hanti: (antisymmetric by_sp)/\(antisymmetric by_dbp)):
-Sorted by_dbp B -> 
-Sorted by_sp A -> 
 Is_uniform (UM B A) B A.
-Proof. intros. 
-       assert(HA:(sort by_sp A) = A).
-       { 
-        apply sort_equal_nodup. apply by_sp_refl. apply Hanti.
-        all: auto. 
-       }
-       assert(HB:(sort by_dbp B)  = B).
-       {
-        apply sort_equal_nodup. apply by_dbp_refl. apply Hanti.
-        all: auto.
-       }
-        unfold UM.
-        rewrite HA.  rewrite HB. 
-        assert(Is_uniform (UM_matching B A) B A).
-        eapply mUM.UM_Is_Matching.
-        eauto. eauto. eauto. eauto.
-        unfold UM_matching in H1.
-        auto.
-Qed.
+Proof. intros. intros. assert(HA:Sorted by_sp (sort by_sp A)).
+       apply sort_correct. apply by_sp_P. apply by_sp_P.
+       intros. assert(HB:Sorted by_dbp (sort by_dbp B)).
+       apply sort_correct. apply by_dbp_P. apply by_dbp_P.
+       split. 
+               { unfold UM. apply replace_column_is_uniform. }
+               { split.
+                 { split. 
+                    { split. 
+                      { unfold All_matchable. intros.
+                         eapply UM_aux_is_Ind_Rat with (B:=(sort by_dbp B)) in HA.
+                        unfold Is_IR in HA. unfold UM in H. apply HA in H.
+                        unfold rational in H. lia. auto.
+                      }
+                      { split.
+                       { intros. unfold UM.
+                         replace (ttqb (replace_column
+                         (UM_aux (sort by_dbp B) (sort by_sp A) 0 0)
+                         (uniform_price (sort by_dbp B) (sort by_sp A))) b) with 
+                         (ttqb (UM_aux (sort by_dbp B) (sort by_sp A) 0 0) b).
+                         apply UM_aux_ttqb. apply idb_sort.
+                         auto. apply ida_sort. auto.
+                         apply replace_column_ttqb.
+                       }
+                       { intros. unfold UM.
+                         replace (ttqa (replace_column
+                         (UM_aux (sort by_dbp B) (sort by_sp A) 0 0)
+                          (uniform_price (sort by_dbp B) (sort by_sp A))) a) with 
+                          (ttqa (UM_aux (sort by_dbp B) (sort by_sp A) 0 0) a).
+                         apply UM_aux_ttqa. apply idb_sort.
+                         auto. apply ida_sort. auto. 
+                         apply replace_column_ttqa.
+                       } 
+                     }
+                   }
+                   { split. unfold UM.
+                     replace (bids_of (replace_column
+                     (UM_aux (sort by_dbp B) (sort by_sp A) 0 0)
+                     (uniform_price (sort by_dbp B) (sort by_sp A)))) with 
+                     (bids_of (UM_aux (sort by_dbp B) (sort by_sp A) 0 0)). 
+                     assert(bids_of (UM_aux (sort by_dbp B) 
+                     (sort by_sp A) 0 0) [<=] (sort by_dbp B)).
+                     apply UM_aux_subset_bidsB. eauto.
+                     apply replace_column_bids.
+                     unfold UM.
+                     replace (asks_of (replace_column
+                     (UM_aux (sort by_dbp B) (sort by_sp A) 0 0)
+                     (uniform_price (sort by_dbp B) (sort by_sp A)))) with 
+                     (asks_of (UM_aux (sort by_dbp B) (sort by_sp A) 0 0)). 
+                     assert(asks_of (UM_aux (sort by_dbp B) 
+                     (sort by_sp A) 0 0) [<=] (sort by_sp A)).
+                     apply UM_aux_subset_asksA. eauto.
+                     apply replace_column_asks.
+                   }
+                }
+                { eapply UM_aux_is_Ind_Rat with (B:=(sort by_dbp B)) in HA.
+                  auto. auto. 
+                }
+             }
+          Qed.
 
 (*This Theorem says that UM is fair matching.*)
-
 Theorem UM_FAIR (B:list Bid)(A:list Ask)
 (NZB: forall b, In b B -> (bq b)>0)
 (NZA: forall a, In a A -> (sq a)>0)
 (NDA:NoDup (idas_of A))
 (NDB:NoDup (idbs_of B))
 (Hanti: (antisymmetric by_sp)/\(antisymmetric by_dbp)):
-Sorted by_dbp B -> 
-Sorted by_sp A -> 
 Is_fair (UM B A) B A.
-Proof. intros. 
-       assert(HA:(sort by_sp A) = A).
-       { 
-        apply sort_equal_nodup. apply by_sp_refl. apply Hanti.
-        all: auto. 
-       }
-       assert(HB:(sort by_dbp B)  = B).
-       {
-        apply sort_equal_nodup. apply by_dbp_refl. apply Hanti.
-        all: auto.
-       }
-        unfold UM.
-        rewrite HA.  rewrite HB. 
-        assert(Is_fair (UM_matching B A) B A).
-        apply UM_Fair. all:auto.
+Proof.  assert(HA:Sorted by_sp (sort by_sp A)).
+                        apply sort_correct. apply by_sp_P. apply by_sp_P.
+                        intros. assert(HB:Sorted by_dbp (sort by_dbp B)).
+                        apply sort_correct. apply by_dbp_P. apply by_dbp_P.
+                        unfold UM. 
+                        assert(Is_fair (UM_matching (sort by_dbp B) (sort by_sp A)) 
+                        (sort by_dbp B) (sort by_sp A)). eapply UM_Fair. apply idb_sort.
+                         auto. apply ida_sort. auto.
+                        auto. auto. unfold UM_matching in H.
+                        apply fair_sort in H. auto.
 Qed.
 
+(*This Theorem says that UM is maximum amongst all the uniform matchings*)
 
 Theorem UM_Maximum (B:list Bid)(A:list Ask)(M:list fill_type)
 (NZB: forall b, In b B -> (bq b)>0)
@@ -117,31 +175,23 @@ Theorem UM_Maximum (B:list Bid)(A:list Ask)(M:list fill_type)
 (NDB:NoDup (idbs_of B))
 (NZT: forall m : fill_type, In m M -> tq m > 0)
 (Hanti: (antisymmetric by_sp)/\(antisymmetric by_dbp)):
-Sorted by_dbp B -> 
-Sorted by_sp A ->
 Is_uniform M B A ->
 QM((UM B A))>=QM(M).
-Proof. intros. 
-       assert(HA:(sort by_sp A) = A).
-       { 
-        apply sort_equal_nodup. apply by_sp_refl. apply Hanti.
-        all: auto. 
-       }
-       assert(HB:(sort by_dbp B)  = B).
-       {
-        apply sort_equal_nodup. apply by_dbp_refl. apply Hanti.
-        all: auto.
-       }
-        unfold UM.
-        rewrite HA.  rewrite HB.
-        replace (QM (replace_column (UM_aux B A 0 0) (uniform_price B A)))
-        with (QM (UM_aux B A 0 0)).
+Proof.  unfold UM. intros.
+        replace (QM (replace_column
+        (UM_aux (sort by_dbp B) (sort by_sp A) 0 0)
+        (uniform_price (sort by_dbp B) (sort by_sp A))))
+        with (QM (UM_aux (sort by_dbp B) (sort by_sp A) 0 0)).
         apply UM_aux_optimal. 
-        all: auto. 
+        all: auto. eauto. eauto. apply ida_sort. auto.
+        apply idb_sort. auto. apply sort_correct.
+        apply by_dbp_P. apply by_dbp_P.
+        apply sort_correct. apply by_sp_P. apply by_sp_P.
+        split. apply H. split. destruct H. destruct H0.
+        apply match_inv with (M':=M)(B':=(sort by_dbp B))(A':=(sort by_sp A)) in H0.
+        auto. auto. eauto. eauto. apply H.
         eapply replace_column_size. 
 Qed.
-
-
 
 End UM_Process.
 
